Finished cms_lookup_insert_diff.

examples/cms/cms.v
@@ -3,6 +3,7 @@ Require Import Coq.ZArith.ZArith.
 Require Import Coq.Lists.List.
 Require Import Coq.Logic.FunctionalExtensionality.
 Require Import Coq.micromega.Lia.
+Require Import VST.zlist.Zlist.
 Import ListNotations.
 
 Generalizable All Variables.
@@ -40,7 +41,7 @@ End DerivedProp.
 
 (* Set Printing All.
 About lookup_insert_diff. *)
-(* 
+(*
 Section Z2Map.
 
   Definition z2map: Type := (Z * Z) -> option Z.
@@ -71,7 +72,7 @@ Section Z2Map.
 End Z2Map. *)
 
 Section CMS.
-  
+
   Context `{M: Map (nat * Z) Z}.
 
   Variable Key: Type.
@@ -80,81 +81,81 @@ Section CMS.
   Variable hash: nat -> Key -> Z.
 
   Definition gen_indexes (k: Key) : list (nat * Z) :=
-    map (fun idx => (idx, hash idx k)) (seq 0 num_rows).  
+    map (fun idx => (idx, hash idx k)) (seq 0 num_rows).
 
   Lemma gen_indexes_length : forall k,
-    length (gen_indexes k) = num_rows.
+      length (gen_indexes k) = num_rows.
   Proof.
     intros. unfold gen_indexes. rewrite map_length. apply seq_length.
   Qed.
 
-  Definition z2lookup_default (k: nat * Z) (m: map_carrier) := 
+  Definition z2lookup_default (k: nat * Z) (m: map_carrier) :=
     match lookup k m with
     | None => 0
     | Some v => v
     end.
 
   Lemma lookup_insert_diff_default: forall k1 k2 v m,
-   k1 <> k2 -> z2lookup_default k1 (insert k2 v m) = z2lookup_default k1 m. 
+      k1 <> k2 -> z2lookup_default k1 (insert k2 v m) = z2lookup_default k1 m.
   Proof.
     intros.
     unfold z2lookup_default.
     rewrite lookup_insert_diff; auto.
   Qed.
-  
+
   Lemma lookup_insert_same_default: forall k v m,
-   z2lookup_default k (insert k v m) = v. 
+      z2lookup_default k (insert k v m) = v.
   Proof.
     intros.
     unfold z2lookup_default.
     rewrite lookup_insert_same; auto.
   Qed.
 
-  Definition cms_insert (k: Key) (m: map_carrier) : map_carrier := 
-    List.fold_left 
+  Definition cms_insert (k: Key) (m: map_carrier) : map_carrier :=
+    List.fold_left
       (fun agg idx => insert idx ((z2lookup_default idx agg) + 1) agg)
       (gen_indexes k) m.
 
   Definition get_hd {A: Type} (l: list A) (H: (length l > 0)%nat): A.
   Proof.
-    refine (( 
-    match l as k return ((length k > 0)%nat -> A) with
-    | nil => fun s => _
-    | a :: _ => fun _ => a
-    end) H).
-    simpl in s. exfalso. apply (gt_irrefl 0). assumption. 
+    refine ((
+               match l as k return ((length k > 0)%nat -> A) with
+               | nil => fun s => _
+               | a :: _ => fun _ => a
+               end) H).
+    simpl in s. exfalso. apply (gt_irrefl 0). assumption.
     (* simpl in s. apply gt_irrefl in s. exfalso. assumption. *)
-    (* trick: define a commplex lemma and then apply to shorten 
+  (* trick: define a commplex lemma and then apply to shorten
               the definition printed out. *)
-  Defined. 
+  Defined.
 
-(*  
+  (*
   Dependent type programming.
   Print get_hd => gives us the definition to replace the above with.
   Lemma test: (length (1::2::3::nil) > 0)%nat.
-  Proof. vm_compute. auto. Qed.  
+  Proof. vm_compute. auto. Qed.
   Compute (get_hd (1::2::3::nil) test). *)
 
-  Definition get_min (l: list Z) (H: (length l > 0)%nat): Z := 
+  Definition get_min (l: list Z) (H: (length l > 0)%nat): Z :=
     List.fold_left Z.min l (get_hd l H).
 
   Lemma fold_left_min_hd: forall l a,
-     fold_left Z.min l a <= a.
-  Proof. 
+      fold_left Z.min l a <= a.
+  Proof.
     induction l; intros; simpl.
     - lia.
     - transitivity (Z.min a0 a); auto. lia.
   Qed.
 
   Lemma fold_left_min_tail: forall l a v,
-    In v l -> fold_left Z.min l a <= v.
+      In v l -> fold_left Z.min l a <= v.
   Proof.
     induction l; intros.
     - inversion H.
     - simpl in *. destruct H.
       + subst v. transitivity (Z.min a0 a); try lia.
         apply fold_left_min_hd.
-      + apply IHl; auto. 
+      + apply IHl; auto.
   Qed.
 
   (*  H(type) depends on l(term) *)
@@ -162,10 +163,10 @@ Section CMS.
   Proof.
     intros. unfold get_min. apply fold_left_min_tail; auto.
   Qed.
-  
+
   Lemma fold_left_min_in: forall l a,
-     fold_left Z.min l a = a \/ In (fold_left Z.min l a) l.
-  Proof. 
+      fold_left Z.min l a = a \/ In (fold_left Z.min l a) l.
+  Proof.
     induction l; intros; simpl.
     - left; auto.
     - destruct (IHl (Z.min a0 a)); auto.
@@ -181,9 +182,9 @@ Section CMS.
     - unfold get_hd. now left.
   Qed.
 
-  Lemma cms_lookup_helper m k: 
-  (length (map (fun idx : nat * Z => z2lookup_default idx m) (gen_indexes k)) >
- 0)%nat.
+  Lemma cms_lookup_helper m k:
+    (length (map (fun idx : nat * Z => z2lookup_default idx m) (gen_indexes k)) >
+       0)%nat.
   Proof.
     rewrite map_length, gen_indexes_length. assumption.
   Qed.
@@ -194,7 +195,7 @@ Section CMS.
   Definition cms_empty : map_carrier := empty.
 
   Lemma get_min_all_zero: forall {A} (f: A -> Z) l H,
-    (forall a, f a = 0) -> get_min (map f l) H = 0.
+      (forall a, f a = 0) -> get_min (map f l) H = 0.
   Proof.
     intros.
     pose proof (get_min_spec_in (map f l) H).
@@ -203,183 +204,152 @@ Section CMS.
       rewrite H0 in H. destruct H; auto.
     }
     apply H2 in H1. assumption.
-  Qed.  
-  
+  Qed.
+
   Lemma cms_lookup_empty: forall k : Key, cms_lookup k cms_empty = 0.
-    Proof. intros. unfold cms_lookup, z2lookup_default, cms_empty.
+  Proof.
+    intros. unfold cms_lookup, z2lookup_default, cms_empty.
     apply get_min_all_zero.
-    intros. rewrite lookup_empty. reflexivity. Qed.
-
-  Lemma lookup_insert_diff_0: forall k1 k2 m,
-    Hash0 k1 <> Hash0 k2 ->
-    z2lookup_default (0, Hash0 k1) (cms_insert k2 m) = 
-    z2lookup_default (0, Hash0 k1) m.
-  Proof.
-    intros. unfold cms_insert. 
-    rewrite !lookup_insert_diff_default; [|intro Hs; inversion Hs..];[|contradiction].
-    auto.
+    intros. rewrite lookup_empty. reflexivity.
   Qed.
 
-  Lemma lookup_insert_diff_1: forall k1 k2 m,
-    Hash1 k1 <> Hash1 k2 ->
-    z2lookup_default (1, Hash1 k1) (cms_insert k2 m) = 
-    z2lookup_default (1, Hash1 k1) m.
+  Lemma fold_left_Zmin_add: forall l a i,
+      fold_left Z.min (map (fun x => Z.add x a) l) (i + a) =
+        fold_left Z.min l i + a.
   Proof.
-    intros. unfold cms_insert. 
-    rewrite !lookup_insert_diff_default; [|intro Hs; inversion Hs..];[|contradiction].
-    auto.
-  Qed.
-
-  Lemma lookup_insert_diff_2: forall k1 k2 m,
-    Hash2 k1 <> Hash2 k2 ->
-    z2lookup_default (2, Hash2 k1) (cms_insert k2 m) = 
-    z2lookup_default (2, Hash2 k1) m.
-  Proof.
-    intros. unfold cms_insert. 
-    rewrite !lookup_insert_diff_default; [|intro Hs; inversion Hs..];[|contradiction].
-    auto.
-  Qed.
-
-  Lemma lookup_insert_same_0: forall k1 k2 m,
-    Hash0 k1 = Hash0 k2 ->
-    z2lookup_default (0, Hash0 k1) (cms_insert k2 m) = 
-    z2lookup_default (0, Hash0 k1) m + 1.
-  Proof.
-    intros. unfold cms_insert. 
-    rewrite 2 lookup_insert_diff_default; [|intro Hs; inversion Hs..].
-    rewrite H. rewrite lookup_insert_same_default.
-    auto.
-  Qed.
-
-  Lemma lookup_insert_same_1: forall k1 k2 m,
-    Hash1 k1 = Hash1 k2 ->
-    z2lookup_default (1, Hash1 k1) (cms_insert k2 m) = 
-    z2lookup_default (1, Hash1 k1) m + 1.
-  Proof.
-    intros. unfold cms_insert. 
-    rewrite lookup_insert_diff_default; [|intro Hs; inversion Hs..].
-    rewrite H. rewrite lookup_insert_same_default.
-    rewrite lookup_insert_diff_default; [|intro Hs; inversion Hs..].
-    auto.
-  Qed.
-
-  Lemma lookup_insert_same_2: forall k1 k2 m,
-    Hash2 k1 = Hash2 k2 ->
-    z2lookup_default (2, Hash2 k1) (cms_insert k2 m) = 
-    z2lookup_default (2, Hash2 k1) m + 1.
-  Proof.
-    intros. unfold cms_insert. 
-    rewrite H. rewrite lookup_insert_same_default.
-    rewrite 2 lookup_insert_diff_default; [|intro Hs; inversion Hs..].
-    auto.
-  Qed.
-
-  Lemma lookup_insert_0: forall k m,
-    z2lookup_default (0, Hash0 k) (cms_insert k m) = z2lookup_default (0, Hash0 k) m + 1.
-  Proof.
-    intros. apply lookup_insert_same_0. (* debug *) auto.
-  Qed.    
-
-  Lemma lookup_insert_1: forall k m,
-    z2lookup_default (1, Hash1 k) (cms_insert k m) = z2lookup_default (1, Hash1 k) m + 1.
-  Proof.
-    intros. apply lookup_insert_same_1. auto.
-  Qed.    
-  
-  Lemma lookup_insert_2: forall k m,
-    z2lookup_default (2, Hash2 k) (cms_insert k m) = z2lookup_default (2, Hash2 k) m + 1.
-  Proof.
-    intros. apply lookup_insert_same_2. auto.
-  Qed.
-
-  Lemma fold_left_Zmin_add: forall l a i, 
-    fold_left Z.min (map (fun x => Z.add x a) l) (i + a) =
-    fold_left Z.min l i + a.
-  Proof.  
     induction l; intros b i; simpl; auto.
     rewrite Z.add_min_distr_r. apply IHl.
-  Qed. 
-
-  Lemma cms_lookup_insert: forall k m, cms_lookup k (cms_insert k m) = cms_lookup k m + 1.
-  Proof. intros. unfold cms_lookup.
-    rewrite lookup_insert_0, lookup_insert_1, lookup_insert_2.
-    remember (z2lookup_default (0, Hash0 k) m) as z0.
-    remember (z2lookup_default (1, Hash1 k) m) as z1.
-    remember (z2lookup_default (2, Hash2 k) m) as z2.
-    rewrite <- fold_left_Zmin_add. simpl map. reflexivity.
   Qed.
 
-  
-  Lemma z2lookup_cms_insert: forall n k1 k2 m, 
-    z2lookup_default (n, hash n k1) (cms_insert k2 m) =
-    z2lookup_default (n, hash n k1) m \/
-    z2lookup_default (n, hash n k1) (cms_insert k2 m) =
-    z2lookup_default (n, hash n k1) m + 1.
+  Lemma cms_lookup_insert: forall k m, cms_lookup k (cms_insert k m) = cms_lookup k m + 1.
+  Proof.
+  Abort.
+
+  Lemma lookup_fold_left_ignore: forall idx f indexes m,
+      ~ In idx indexes ->
+      (forall j1 j2 m', j1 <> j2 -> z2lookup_default j1 (f m' j2) = z2lookup_default j1 m') ->
+      z2lookup_default idx (fold_left f indexes m) = z2lookup_default idx m.
+  Proof.
+    intros idx f indexes m Hn Hf. revert dependent indexes. intro.
+    apply rev_ind with (l := indexes); intros; simpl; auto.
+    rewrite fold_left_app. simpl. rewrite Hf.
+    - rewrite H; auto. intuition.
+    - intro. apply Hn. rewrite in_app_iff. right. subst. intuition.
+  Qed.
+
+  Lemma not_in_hash_seq: forall k1 k2 n l, ~ In n l -> ~ In (n, hash n k1) (map (fun idx : nat => (idx, hash idx k2)) l).
+  Proof.
+    intros k1 k2 n. induction l; intros; simpl; auto. simpl in H.
+    apply Decidable.not_or in H. destruct H. specialize (IHl H0). intro. destruct H1.
+    - apply H. inversion H1; auto.
+    - contradiction.
+  Qed.
+
+  Lemma z2lookup_cms_insert: forall n k1 k2 m,
+      z2lookup_default (n, hash n k1) (cms_insert k2 m) =
+        z2lookup_default (n, hash n k1) m \/
+        z2lookup_default (n, hash n k1) (cms_insert k2 m) =
+          z2lookup_default (n, hash n k1) m + 1.
   Proof.
     intros. destruct (le_lt_dec num_rows n).
     - left. unfold cms_insert. unfold gen_indexes. clear num_rows_pos.
-      induction num_rows.
-      + simpl. reflexivity.
-      + assert (map (fun idx : nat => (idx, hash idx k2)) (seq 0 (S n0)) = 
-          (map (fun idx : nat => (idx, hash idx k2)) (seq 0 n0)) ++ [(n0, hash n0 k2)]). {
-            replace (S n0) with (n0 + 1)%nat by lia.
-            rewrite seq_app, map_app. f_equal. }
-        rewrite H. rewrite fold_left_app.
-        remember (fold_left
-            (fun (agg : map_carrier) (idx : nat * Z) =>
-             insert idx (z2lookup_default idx agg + 1) agg)
-            (map (fun idx : nat => (idx, hash idx k2)) (seq 0 n0)) m).
-            simpl.
+      rewrite lookup_fold_left_ignore; auto.
+      + apply not_in_hash_seq. rewrite in_seq. lia.
+      + intros. apply lookup_insert_diff_default. auto.
+    - destruct (Z.eq_dec (hash n k1) (hash n k2)); [right | left].
+      + unfold cms_insert. unfold gen_indexes.
+        replace num_rows with (n + (num_rows - n))%nat by lia.
+        rewrite seq_app, map_app, fold_left_app. simpl.
+        replace (num_rows - n)%nat with (1 + (num_rows - n - 1))%nat by lia.
+        rewrite seq_app, map_app, fold_left_app. simpl.
+        rewrite lookup_fold_left_ignore.
+        3: intros; apply lookup_insert_diff_default; auto.
+        2: apply not_in_hash_seq; rewrite in_seq; lia.
+        rewrite e. rewrite lookup_insert_same_default.
+        rewrite lookup_fold_left_ignore; auto.
+        * apply not_in_hash_seq; rewrite in_seq; lia.
+        * intros; apply lookup_insert_diff_default; auto.
+      + unfold cms_insert. unfold gen_indexes.
+        replace num_rows with (n + (num_rows - n))%nat by lia.
+        rewrite seq_app, map_app, fold_left_app. simpl.
+        replace (num_rows - n)%nat with (1 + (num_rows - n - 1))%nat by lia.
+        rewrite seq_app, map_app, fold_left_app. simpl.
+        rewrite lookup_fold_left_ignore.
+        3: intros; apply lookup_insert_diff_default; auto.
+        2: apply not_in_hash_seq; rewrite in_seq; lia.
+        rewrite lookup_insert_diff_default. 2: intro Hs; inversion Hs; contradiction.
+        rewrite lookup_fold_left_ignore; auto.
+        * apply not_in_hash_seq; rewrite in_seq; lia.
+        * intros; apply lookup_insert_diff_default; auto.
   Qed.
-  Lemma cms_lookup_insert_diff: forall k1 k2 m, 
-      cms_lookup k2 (cms_insert k1 m) = cms_lookup k2 m \/ 
-      cms_lookup k2 (cms_insert k1 m) = cms_lookup k2 m + 1.
+
+  Definition min_in_list (l: list Z) (a: Z) : Prop := In a l /\ (forall v, In v l -> a <= v).
+
+  Lemma min_unique: forall l v1 v2, min_in_list l v1 -> min_in_list l v2 -> v1 = v2.
+  Proof.
+    intros. destruct H, H0. apply H1 in H0. apply H2 in H. lia.
+  Qed.
+
+  Lemma get_min_cons_nonempty: forall a l H Hl, get_min (a :: l) H = Z.min a (get_min l Hl).
   Proof.
     intros.
-    unfold cms_lookup.
+    assert (min_in_list (a :: l) (get_min (a :: l) H)). {
+      split. apply get_min_spec_in. intro; apply get_min_spec_ineq; auto. }
+    assert (min_in_list (a :: l) (Z.min a (get_min l Hl))). {
+      split; intros.
+      - destruct (Z.min_spec a (get_min l Hl)) as [[] | []]; rewrite H2.
+        + now left.
+        + right. apply get_min_spec_in.
+      - simpl in H1. destruct H1.
+        + subst. lia.
+        + pose proof (get_min_spec_ineq l v Hl H1). lia. }
+    eapply min_unique; eauto.
+  Qed.
 
-    destruct ((Hash0 k1 =? Hash0 k2)) eqn:Hh0;
-    destruct (Z.eqb (Hash1 k1) (Hash1 k2)) eqn:Hh1;
-    destruct (Z.eqb (Hash2 k1) (Hash2 k2)) eqn:Hh2.
-    - rewrite Z.eqb_eq in *.
-      right.
-      unfold cms_lookup.
-      rewrite <- Hh0.
-      rewrite <- Hh1.
-      rewrite <- Hh2.
-      rewrite lookup_insert_0, lookup_insert_1, lookup_insert_2.
-      rewrite <- fold_left_Zmin_add. reflexivity.
-    - rewrite Z.eqb_eq in *.
-      right.
-      unfold cms_lookup.
-      rewrite <- Hh0.
-      rewrite <- Hh1.
-      rewrite lookup_insert_0, lookup_insert_1.
-      rewrite lookup_insert_diff_2.
-      
+  Lemma list_diff_at_most_one: forall (l1 l2: list Z) H1 H2,
+      length l1 = length l2 ->
+      (forall i, (0 <= i < length l1)%nat -> nth i l1 0 = nth i l2 0 \/ nth i l1 0 = nth i l2 0 + 1) ->
+      get_min l1 H1 = get_min l2 H2 \/ get_min l1 H1 = get_min l2 H2 + 1.
+  Proof.
+    induction l1; intros.
+    - destruct l2. simpl in H1; lia. simpl in H. lia.
+    - destruct l2. simpl in H2; lia.
+      destruct (zerop (length l1)), (zerop (length l2)); try (simpl in H; lia).
+      + destruct l1, l2; simpl in H; try lia. 2: simpl in e, e0; lia.
+        unfold get_min. simpl. specialize (H0 O ltac:(lia)). simpl in H0. lia.
+      + assert (length l1 > 0)%nat by lia. assert (length l2 > 0)%nat by lia.
+        rewrite (get_min_cons_nonempty a l1 _ H3). rewrite (get_min_cons_nonempty z l2 _ H4).
+        pose proof (H0 O ltac:(lia)). simpl in H5.
+        assert (forall i : nat,
+                   (0 <= i < length l1)%nat -> nth i l1 0 = nth i l2 0 \/ nth i l1 0 = nth i l2 0 + 1). {
+          intros. simpl length in H0. specialize (H0 (S i)%nat ltac:(lia)). simpl in H0. assumption.
+        }
+        specialize (IHl1 l2 H3 H4 ltac:(simpl in H; lia) H6). lia.
+  Qed.
 
+  Lemma cms_lookup_insert_diff: forall k1 k2 m,
+      cms_lookup k2 (cms_insert k1 m) = cms_lookup k2 m \/
+        cms_lookup k2 (cms_insert k1 m) = cms_lookup k2 m + 1.
+  Proof.
+    intros.
+    unfold cms_lookup. apply list_diff_at_most_one.
+    - rewrite !map_length. easy.
+    - rewrite map_length. intros.
+      rewrite !nth_map' with (d' := (O, 0)); try lia.
+      assert (nth i (gen_indexes k2) (0%nat, 0) = (i, hash i k2)). {
+        unfold gen_indexes. rewrite nth_map' with (d' := O).
+        - rewrite seq_nth. reflexivity. unfold gen_indexes in H.
+          rewrite map_length, seq_length in H. lia.
+        - rewrite seq_length. rewrite gen_indexes_length in H. lia.
+      }
+      rewrite H0.
+      apply z2lookup_cms_insert.
+  Qed.
 
-    2: { left. unfold cms_lookup.
-    apply Z.eqb_eq in Hh0.
-    rewrite <- Hh0.
-
-    lookup
-    rewrite lookup_insert0, lookup_insert1, lookup_insert2.
-    remember (z2lookup_default (0, Hash0 k) m) as z0.
-    remember (z2lookup_default (1, Hash1 k) m) as z1.
-    remember (z2lookup_default (2, Hash2 k) m) as z2.
-
-
-    }
-
-
-  Admitted.
-
-  Lemma cms_insert_comm: forall k1 k2 m, 
+  Lemma cms_insert_comm: forall k1 k2 m,
       cms_insert k1 (cms_insert k2 m) = cms_insert k2 (cms_insert k1 m).
   Proof.
     intros.
-    apply functional_extensionality.
-    
+  Abort.
 
 End CMS.
